Automated refinement is largely working

Refine.v
@@ -5,26 +5,35 @@ Require Import Coq.Program.Program.
 Require Import Fiat.ADTRefinement.
 Require Import Fiat.ADTRefinement.BuildADTRefinements.
 
-Definition comp_rel (X X' : Type) (AbsR : rel X X') : rel (Comp X) (Comp X') :=
-  fun cX cX' => (forall x,  cX  x  -> exists x', AbsR x x' /\ cX' x') /\
-                (forall x', cX' x' -> exists x,  AbsR x x' /\ cX  x).
+Lemma If_Then_Else_fst : forall p A B (a b : A * B),
+  fst (If p Then a Else b) = If p Then (fst a) Else (fst b).
+Proof. intros; destruct p; trivial. Qed.
 
-Theorem refine_rel (X X' : Type)
-        (AbsR : rel X X') f f' g g'
-  (functional : forall x y z, AbsR x y -> AbsR x z -> y = z) :
-  Related f f' (comp_rel AbsR) ->
-  Related g g' (comp_rel AbsR) ->
-  refine f g -> refine f' g'.
-Proof.
-  repeat intro.
-  destruct H0.
-  destruct (H3 v H2) as [? [? ?]].
-  destruct H.
-  specialize (H1 x H5).
-  destruct (H x H1) as [? [? ?]].
-  pose proof (functional _ _ _ H4 H7); subst.
-  apply H8.
-Qed.
+Lemma If_Then_Else_snd : forall p A B (a b : A * B),
+  snd (If p Then a Else b) = If p Then (snd a) Else (snd b).
+Proof. intros; destruct p; trivial. Qed.
+
+Class RelatedTheory {A B : Type} (x : A) (AbsR : A -> B -> Prop) := {
+  translation : B;
+  relationship : Related x translation AbsR
+}.
+
+Arguments relationship {_ _ _ _ _} /.
+
+Program Instance RelatedTheory_AbsR {A B : Type} (x : A) (y : B)
+        (AbsR : A -> B -> Prop) : Related x y AbsR ->
+  RelatedTheory x AbsR := {
+  translation := y
+}.
+
+Notation "translation[ H ]" := (@translation _ _ _ _ H)
+  (at level 9, format "translation[ H ]").
+Notation "relationship[ H ]" := (@relationship _ _ _ _ H)
+  (at level 9, format "relationship[ H ]").
+
+Corollary rewrite_rel `{AbsR : rel X Y} {x : X} {y : Y} :
+  AbsR x y -> Related x y AbsR.
+Proof. intro H; apply H. Qed.
 
 Section Refine.
 
@@ -44,7 +53,6 @@ Definition spec : ADT _ := Def ADT {
 
   Def Method1 "delete" (r : rep) (x : A) : rep * unit :=
     ret (Subtract _ r x, tt)
-
 }%ADTParsing.
 
 Variable A_eq_dec : forall x y : A, {x = y} + {x <> y}.
@@ -53,18 +61,11 @@ Definition EnsembleAsList_AbsR : rel (Ensemble A) (list A) :=
   fun r_o r_n =>
     forall x, In _ r_o x <-> List.existsb (A_eq_dec x) r_n.
 
-Class RelatedTheory {A B : Type} (x : A) (AbsR : A -> B -> Prop) := {
-  translation : B;
-  relationship : Related x translation AbsR
+Program Instance RelatedTheory_Empty_set :
+  RelatedTheory (Empty_set A) EnsembleAsList_AbsR := {
+  translation := []
 }.
-
-Arguments relationship {_ _ _ _ _} /.
-
-Program Instance RelatedTheory_AbsR {A B : Type} (x : A) (y : B)
-        (AbsR : A -> B -> Prop) : Related x y AbsR ->
-  RelatedTheory x AbsR := {
-  translation := y
-}.
+Next Obligation. intro x; split; inversion 1. Qed.
 
 Program Instance RelatedTheory_decides_In {es : Ensemble A} (d : A) :
   RelatedTheory es EnsembleAsList_AbsR ->
@@ -127,25 +128,42 @@ Next Obligation.
       constructor.
 Admitted.
 
-Corollary rewrite_rel `{AbsR : rel X Y} {x : X} {y : Y} :
-  AbsR x y -> Related x y AbsR.
-Proof. intro H; apply H. Qed.
+Program Instance RelatedTheory_If_Then_Else
+        (b : bool) (t e : Ensemble A)
+        (Ht : RelatedTheory t EnsembleAsList_AbsR)
+        (He : RelatedTheory e EnsembleAsList_AbsR) :
+  RelatedTheory (If b Then t Else e) EnsembleAsList_AbsR := {
+  translation := if b then translation[Ht]
+                      else translation[He]
+}.
+Next Obligation.
+  intro x; split; intros;
+  destruct Ht, He; simpl in *;
+  unfold Related in *; subst;
+  destruct b; simpl in *;
+  try apply relationship0;
+  try apply relationship1;
+  assumption.
+Qed.
 
 Ltac translate :=
-  try match goal with
-  | [ H : ?R _ _ |- refine (_ <- ?X; _) _ ] =>
-    apply rewrite_rel in H;
+  match goal with
+  | [ |- refine (ret _) _ ] => solve [ finish honing ]
+  | [ H : Related _ _ _ |- refine { x : _ | ?R ?X x } _ ] =>
+    refine pick val (@translation _ _ X R _); [|try apply relationship];
+    simpl; try simplify with monad laws; translate
+  | [ H : Related _ _ _ |- refine (_ <- { x : _ | ?R ?X x }; _) _ ] =>
+    refine pick val (@translation _ _ X R _); [|try apply relationship];
+    simpl; try simplify with monad laws; translate
+  | [ H : Related _ _ _ |- refine (_ <- ?X; _) _ ] =>
     rewrite (@relationship _ _ X _ _); simpl;
-    try simplify with monad laws; translate
-  end.
-
-Lemma If_Then_Else_fst : forall p A B (a b : A * B),
-  fst (If p Then a Else b) = If p Then (fst a) Else (fst b).
-Proof. intros; destruct p; trivial. Qed.
-
-Lemma If_Then_Else_snd : forall p A B (a b : A * B),
-  snd (If p Then a Else b) = If p Then (snd a) Else (snd b).
-Proof. intros; destruct p; trivial. Qed.
+    simpl; try simplify with monad laws; translate
+  | [ |- refine { x : _ | ?R ?X x } _ ] =>
+    refine pick val (@translation _ _ X R _); [|try apply relationship];
+    simpl; try simplify with monad laws; translate
+  | [ H : Related _ _ _ |- _ ] => idtac
+  | [ H : ?R _ _ |- _ ] => apply rewrite_rel in H; translate
+  end; simpl.
 
 Theorem impl : FullySharpened spec.
 Proof.
@@ -153,36 +171,18 @@ Proof.
   hone representation using EnsembleAsList_AbsR;
 
   (* See if our known theories can resolve things for us. *)
-  try simplify with monad laws; simpl;
-  try translate.
-
-  (* constructor: new *)
-  {
-    (* NOTE: Although [finish honing] might solve this goal directly, it
-      would generate a new subgoal at the end (from the call to
-      [finish_SharpeningADT_WithoutDelegation]), requiring us to prove that
-      [Empty_set] is equivalent to an empty list. Thus, the objective in
-      these proofs is not just to complete the subgoals, but to reduce the
-      goal to its simplest possible form, expressed purely in terms of our
-      concrete representation (in this case, lists). *)
-
-    refine pick val nil.
-      finish honing.
-    split; intros;
-    inversion H0.
-  }
+  try simplify with monad laws; try translate.
 
   {
     rewrite refine_If_Then_Else_ret;
     simplify with monad laws; simpl.
     rewrite If_Then_Else_fst; simpl.
-    apply rewrite_rel in H0.
-    rewrite (@relationship _ _ {b : bool | decides b (In A r_o d)} _ _).
-    unfold Related in H1.
-    rewrite H1.
-    unfold translation; simpl.
-    simpl in X.
-    remember {b : bool | decides b (In A r_o d)} as p.
+    translate.
+    rewrite If_Then_Else_snd; simpl.
+    replace (If List.existsb (A_eq_dec d) r_n Then () Else ()) with ()
+      by (destruct (List.existsb _ _); auto).
+    finish honing.
+  }
 
   finish_SharpeningADT_WithoutDelegation.
 Defined.
