Notes.v
@@ -1,0 +1,20 @@
+Definition comp_rel (X X' : Type) (AbsR : rel X X') : rel (Comp X) (Comp X') :=
+  fun cX cX' => (forall x,  cX  x  -> exists x', AbsR x x' /\ cX' x') /\
+                (forall x', cX' x' -> exists x,  AbsR x x' /\ cX  x).
+
+Theorem refine_rel (X X' : Type)
+        (AbsR : rel X X') f f' g g'
+  (functional : forall x y z, AbsR x y -> AbsR x z -> y = z) :
+  Related f f' (comp_rel AbsR) ->
+  Related g g' (comp_rel AbsR) ->
+  refine f g -> refine f' g'.
+Proof.
+  repeat intro.
+  destruct H0.
+  destruct (H3 v H2) as [? [? ?]].
+  destruct H.
+  specialize (H1 x H5).
+  destruct (H x H1) as [? [? ?]].
+  pose proof (functional _ _ _ H4 H7); subst.
+  apply H8.
+Qed.
